Hoare/Logic.thy
@@ -1,0 +1,286 @@
+theory Logic imports "../Yul/YulSemanticsSingleStep"
+begin
+
+definition YulSteps ::
+  "('g, 'v, 't) YulDialect \<Rightarrow>
+  (('g, 'v, 't) result \<Rightarrow> bool) \<Rightarrow>
+   (('g, 'v, 't) result \<Rightarrow> bool) \<Rightarrow>
+   bool" 
+("_ % {_} {_}")
+  where
+"YulSteps D P Q =
+  (\<forall> st . P st \<longrightarrow>
+    (\<exists> n st' . evalYul' D st n = YulResult st' \<and>
+     Q st'))"
+
+lemma YSI [intro]:
+  assumes
+    "\<And> st . P st \<Longrightarrow> 
+      (\<exists> n st' . evalYul' D st n = YulResult st' \<and>
+     Q st')"
+  shows "D % {P} {Q}" using assms
+  unfolding YulSteps_def 
+  by auto
+
+lemma HTE [elim]:
+  assumes H : "D%{P} {Q}"
+  assumes HP : "P st"
+  shows "(\<exists> n st'. evalYul' D st n = YulResult st' \<and>
+     Q st')"
+  using assms unfolding YulSteps_def by auto
+
+(* Hoare logic rules *)
+lemma HT_conseq :
+  assumes H : "D%{P} {Q}"
+  assumes HP : "\<And> st . P' st \<Longrightarrow> P st"
+  assumes HQ : "\<And> st . Q st \<Longrightarrow> Q' st"
+  shows "D%{P'} {Q'}"
+proof
+  fix st
+  assume P' : "P' st"
+  hence P : "P st" using HP by auto
+
+  obtain n st' where Exec : "evalYul' D st n = YulResult st' \<and> 
+           Q st'"
+    using HTE[OF H P] by auto
+
+  hence Q' : "Q' st'" using HQ Exec by auto
+
+  thus "\<exists>n st'.
+             evalYul' D st n = YulResult st' \<and> Q' st'"
+    using Exec by blast
+qed
+
+
+lemma HT_step :
+  assumes H : "\<And> st . P st \<Longrightarrow> 
+      (\<exists> st' . evalYulStep D st = YulResult st' \<and> Q st')"
+  shows "D%{P} {Q}"
+proof
+  fix st
+  assume P : "P st"
+  obtain st' where St' : "evalYulStep D st = YulResult st'"  and Q : "Q st'"
+    using H[OF P] by auto
+
+  hence "evalYul' D st 1 = YulResult st'" by auto
+
+  thus "\<exists>n st' . evalYul' D st n = YulResult st' \<and>  Q st'" using St' Q by blast
+qed
+
+lemma evalYul'_steps :
+  assumes H1 : "evalYul' D st1 n1 = YulResult st2"
+  assumes H2 : "evalYul' D st2 n2 = st3"
+  shows "evalYul' D st1 (n1 + n2) = st3" using assms
+proof(induction n1 arbitrary: st1 st2 n2 st3)
+  case 0
+  then show ?case by auto
+next
+  case (Suc n1)
+  show ?case
+  proof(cases "cont st1")
+    case Nil
+    then show ?thesis using Suc by(auto)
+  next
+    case (Cons ch1 ct1)
+
+    obtain st1' where "evalYulStep D st1 = YulResult st1'"
+      using Suc.prems Cons by(auto simp del: evalYulStep.simps split:YulResult.splits)    
+
+    then show ?thesis using Suc.prems Suc.IH Cons
+      by(simp del: evalYulStep.simps)
+  qed
+qed
+
+lemma HT_steps :
+  assumes H1 : "D % {P1} {P2}"
+  assumes H2 : "D % {P2} {P3}"
+  shows "D % {P1} {P3}"
+proof
+  fix st1
+  assume P1 : "P1 st1"
+  obtain n1 st2 where Exec1 : "evalYul' D st1 n1 = YulResult st2" and P2 : "P2 st2"
+    using HTE[OF H1 P1] by auto
+  obtain n2 st3 where Exec2 : "evalYul' D st2 n2 = YulResult st3" and P3 : "P3 st3"
+    using HTE[OF H2 P2] by auto
+
+  have Exec : "evalYul' D st1 (n1 + n2) = YulResult st3"
+    using evalYul'_steps[OF Exec1 Exec2] by auto
+
+  thus "\<exists>n st'. evalYul' D st1 n = YulResult st' \<and> P3 st'" using P3 by blast
+qed
+
+(* characterize successfully halted states *)
+definition is_halted :: "('g, 'v, 't) result \<Rightarrow> bool" where
+"is_halted r = (cont r = [])"
+
+(* a more familiar-looking Hoare logic of statements - but showing its relationship to the
+   actual executions beyond the first instruction will take some work. *)
+definition YulStepsStmt ::
+  "('g, 'v, 't) YulDialect \<Rightarrow>
+   (('g, 'v, 't) result \<Rightarrow> bool) \<Rightarrow>
+   ('v, 't) YulStatement \<Rightarrow>
+   (('g, 'v, 't) result \<Rightarrow> bool) \<Rightarrow>
+   bool" 
+("_ % {_} _ {_}") where
+"(D % {P} c {Q}) =
+  ((D % {P} {Q}) \<and>
+   (\<forall> st . P st \<longrightarrow> cont st = [EnterStatement c]))"
+
+
+(* Revisiting the implementation - how can we make it easier to model behavior?
+   1: formalize continuation stack transformation patterns. everything except for
+break and continue will add a (possibly empty) prefix to the stack, and drop the current element.
+*)
+
+(* one idea: we could have a
+delta function that precisely describes the
+change to the continuation *)
+
+lemma evalYulStep_cont_pref :
+  assumes Hcont : "cont st = h#t"
+  assumes Hstep : "evalYulStep D st = YulResult st'"
+  shows "\<exists> pre . cont st' = pre @ t" 
+proof(cases h)
+  case (EnterStatement st)
+  show ?thesis
+  proof(cases st)
+    case (YulFunctionCallStatement x)
+    then show ?thesis using assms EnterStatement
+      by(cases x; auto)
+  next
+    case (YulAssignmentStatement x)
+    then show ?thesis using assms EnterStatement
+      by(cases x; auto)
+  next
+    case (YulVariableDeclarationStatement x)
+    show ?thesis
+    proof(cases x)
+      case (YulVariableDeclaration x1 x2)
+      then show ?thesis using assms EnterStatement YulVariableDeclarationStatement 
+        by(cases x2; auto)
+    qed
+  next
+    case (YulFunctionDefinitionStatement x)
+    then show ?thesis using assms EnterStatement YulFunctionDefinitionStatement
+      by(auto)
+  next
+    case (YulIf x1 x2)
+    then show ?thesis using assms EnterStatement by auto
+  next
+    case (YulSwitch x1 x2)
+    then show ?thesis using assms EnterStatement by auto
+  next
+    case (YulForLoop pre cond post body)
+    then show ?thesis using assms EnterStatement 
+      by(cases pre; auto)
+  next
+  case YulBreak
+  then show ?thesis using assms EnterStatement
+    by(auto)
+  next
+    case YulContinue
+    then show ?thesis using assms EnterStatement
+      by auto
+  next
+    case YulLeave
+    then show ?thesis using assms EnterStatement
+      by auto
+  next
+    case (YulBlock x11)
+    then show ?thesis using assms EnterStatement
+      by(auto split: sum.splits)
+  qed
+next
+  case (ExitStatement st locals sigs)
+  show ?thesis
+  proof(cases st)
+    case (YulFunctionCallStatement x)
+    then show ?thesis using assms ExitStatement
+      by(cases x; auto split:list.splits)
+  next
+    case (YulAssignmentStatement x)
+    then show ?thesis using assms ExitStatement
+      by(cases x; auto split:list.splits if_splits option.splits)
+  next
+    case (YulVariableDeclarationStatement x)
+    show ?thesis
+    proof(cases x)
+      case (YulVariableDeclaration x1 x2)
+      then show ?thesis using assms ExitStatement YulVariableDeclarationStatement 
+        by(cases x2; auto split: if_splits option.splits)
+    qed
+  next
+    case (YulFunctionDefinitionStatement x) 
+    then show ?thesis using assms ExitStatement YulFunctionDefinitionStatement
+      by(auto)
+  next
+    case (YulIf x1 x2)
+    then show ?thesis using assms ExitStatement
+      by(auto split:list.splits if_splits)
+  next
+    case (YulSwitch x1 x2)
+    then show ?thesis using assms ExitStatement
+      by(auto split:list.splits if_splits prod.splits option.splits YulSwitchCase.splits YulLiteral.splits)
+  next
+    case (YulForLoop x1 x2 x3 x4)
+    then show ?thesis using assms ExitStatement
+      by(auto split:list.splits if_splits)
+  next
+    case YulBreak
+    then show ?thesis using assms ExitStatement
+      apply(auto split:list.splits if_splits)
+  next
+    case YulContinue
+    then show ?thesis sorry
+  next
+    case YulLeave
+    then show ?thesis sorry
+  next
+    case (YulBlock x11)
+    then show ?thesis sorry
+  qed
+    
+next
+  case (EnterFunctionCall x31 x32)
+  then show ?thesis sorry
+next
+  case (ExitFunctionCall x41 x42 x43 x44 x45)
+  then show ?thesis sorry
+next
+  case (Expression x5)
+  then show ?thesis sorry
+qed
+
+
+(* reasoning about Seq. idea:
+   - EnterStatement (spre  @ spost) becomes
+   - (map statement spre) @ (map statement spost)   
+*)
+
+(*
+  another perspective. suppose P \<Longrightarrow> cont = h#t
+  and also Q1 \<Longrightarrow> cont = t
+
+  then. if (P, Q1) holds and (Q1, Q2) holds, then so does
+  (P, Q2) (i.e., extending execution
+
+  this is a special case of ht_steps. but could be a useful
+  notion for reasoning about individual statements.
+
+*)
+
+(*
+lemma evalYul'_bisect_cont :
+  assumes H :
+*)
+
+(* 
+  relating terminating sub-executions
+*)
+
+(*
+  P1 P2 (? ?)
+
+*)
+
+end
